consistency

experiments/DeeperShallowEmbedding.fst
@@ -49,17 +49,6 @@ let app e1 e2 = fun c -> (e1 c) (e2 c)
 
 
 (** Deeper shallow embedding - Figure 3 **)
-noeq
-type dctx : (cs:ctx u#a) -> Type u#(a+1) =
-| Empty : dctx empty_ctx
-| Extend : (#cs:ctx) -> dctx cs -> t:(typ cs) -> dctx (cons cs t)
-
-noeq
-type dvar : #cs:ctx u#a -> dcs:(dctx cs) -> t:(typ cs) -> var cs t -> Type u#(a+1) =
-| Same : #cs:ctx -> #t:typ cs -> #dcs:dctx cs -> dvar (Extend dcs t) (weakenT t) same
-| Next : #cs:ctx -> #dcs:dctx cs -> #t:typ cs -> #at:_ -> #s:_ -> dvar #cs dcs at s -> dvar (Extend dcs t) (weakenT at) (next s)
-
-
 let typ0 (cs:ctx u#4) : Type u#4 = cs -> Type u#0
 let typ1 (cs:ctx u#4) : Type u#4 = cs -> Type u#1
 let typ2 (cs:ctx u#4) : Type u#4 = cs -> Type u#2
@@ -90,11 +79,31 @@ val dt1 : #cs:ctx u#4 -> at:(typ1 cs) -> bt:(typ1 (cons cs (lift1 at))) -> typ1 
 let dt1 #cs at bt = fun (c:cs) -> ((a : at c) -> bt (| c, raise_val a |))
 
 noeq
+type dctx : (cs:ctx u#a) -> Type u#(a+1) =
+| Empty : dctx empty_ctx
+| Extend : (#cs:ctx) -> dctx cs -> t:(typ cs) -> dctx (cons cs t)
+
+noeq
+type dvar : #cs:ctx u#a -> dcs:(dctx cs) -> t:(typ cs) -> var cs t -> Type u#(a+1) =
+| Same : #cs:ctx -> #t:typ cs -> #dcs:dctx cs -> dvar (Extend dcs t) (weakenT t) same
+| Next : #cs:ctx -> #dcs:dctx cs -> #t:typ cs -> #at:_ -> #s:_ -> dvar #cs dcs at s -> dvar (Extend dcs t) (weakenT at) (next s)
+
+noeq
 type dterm : #cs:ctx u#4 -> dcs:dctx cs -> t:typ cs -> term cs t -> Type u#5 =
 | Lambda : #cs:ctx -> #dcs:dctx cs -> #at:typ cs -> #bt:typ (cons cs at) -> #s:_ -> dterm (Extend dcs at) bt s -> dterm dcs (dt at bt) (lambda s)
-| Var : #cs:ctx -> #dcs:dctx cs -> #t:typ cs -> #s:term cs t -> dvar dcs t s -> dterm #cs dcs t s
-| App : #cs:ctx -> #dcs:dctx cs -> #at:typ cs -> #bt:typ (cons cs at) -> #s1:_ -> #s2:_ -> dterm dcs (dt at bt) s1 -> x:(dterm dcs at s2) -> dterm dcs (fun c -> bt (| c, s2 c |)) (app s1 s2)
-| Dt0 : #cs:ctx -> #dcs:dctx cs -> #at:typ0 cs -> #bt:_ -> dterm dcs (lift1 u0) (vlift0 at) -> dterm (Extend dcs (lift0 at)) (lift1 u0) (vlift0 bt) -> dterm dcs (lift1 u0) (vlift0 (dt0 at bt))
-| Dt1 : #cs:ctx -> #dcs:dctx cs -> #at:typ1 cs -> #bt:_ -> dterm dcs (lift2 u1) (vlift1 at) -> dterm (Extend dcs (lift1 at)) (lift2 u1) (vlift1 bt) -> dterm dcs (lift2 u1) (vlift1 (dt1 at bt))
-| U0 : #cs:ctx -> #dcs:dctx cs -> dterm dcs (lift2 u1) (vlift1 u0)
-| U1 : #cs:ctx -> #dcs:dctx cs -> dterm dcs (lift3 u2) (vlift2 u1)
+| Var    : #cs:ctx -> #dcs:dctx cs -> #t:typ cs -> #s:term cs t -> dvar dcs t s -> dterm #cs dcs t s
+| App    : #cs:ctx -> #dcs:dctx cs -> #at:typ cs -> #bt:typ (cons cs at) -> #s1:_ -> #s2:_ -> dterm dcs (dt at bt) s1 -> x:(dterm dcs at s2) -> dterm dcs (fun c -> bt (| c, s2 c |)) (app s1 s2)
+| Dt0    : #cs:ctx -> #dcs:dctx cs -> #at:typ0 cs -> #bt:_ -> dterm dcs (lift1 u0) (vlift0 at) -> dterm (Extend dcs (lift0 at)) (lift1 u0) (vlift0 bt) -> dterm dcs (lift1 u0) (vlift0 (dt0 at bt))
+| Dt1    : #cs:ctx -> #dcs:dctx cs -> #at:typ1 cs -> #bt:_ -> dterm dcs (lift2 u1) (vlift1 at) -> dterm (Extend dcs (lift1 at)) (lift2 u1) (vlift1 bt) -> dterm dcs (lift2 u1) (vlift1 (dt1 at bt))
+| U0     : #cs:ctx -> #dcs:dctx cs -> dterm dcs (lift2 u1) (vlift1 u0)
+| U1     : #cs:ctx -> #dcs:dctx cs -> dterm dcs (lift3 u2) (vlift2 u1)
+
+
+val identity : dterm Empty (dt (lift1 u0) (lift1 u0)) (lambda (lookup same))
+let identity = Lambda (Var Same)
+
+val extract : #cs:ctx -> #dcs:dctx cs -> #at:typ cs -> #a:term cs at -> dterm dcs at a -> term cs at
+let extract #cs #dcs #at #a e = a
+
+val consistency : #t:_ -> dterm #empty_ctx Empty (fun _ -> raise_t u#0 u#4 empty) t -> raise_t u#0 u#4 empty
+let consistency e = (extract e) (raise_val ())
